pulse/lib/pulse/core/PulseCore.BaseHeapSig.fsti
@@ -7,11 +7,13 @@ val base_heap : heap_sig u#a
 val core_ghost_ref_as_addr (_:core_ghost_ref) : GTot nat
 val select_ghost (i:nat) (m:(base_heap u#a).sep.core) : GTot (option (H.cell u#a))
 val ghost_ctr (b:base_heap.mem) : GTot nat
-val mem_invariant_interp (ex:inames base_heap) (h:base_heap.mem)
-: Lemma (interpret (base_heap.mem_invariant ex h) h <==>
-         (forall addr.
-            addr >= ghost_ctr h ==>
-            None? (select_ghost addr (core_of h))))
+let free_above_ghost_ctr (m:base_heap.mem)
+: prop
+= forall addr. addr >= ghost_ctr m ==> select_ghost addr (core_of m) == None
+
+val mem_invariant_interp (ex:inames base_heap) (h0:base_heap.mem) (h1:base_heap.sep.core)
+: Lemma (base_heap.interp (base_heap.mem_invariant ex h0) h1 ==>
+         free_above_ghost_ctr h0)
 val inames_ok_trivial (ex:inames base_heap) (h:base_heap.mem)
 : Lemma (inames_ok ex h)
 
@@ -44,15 +46,46 @@ val ghost_pts_to_compatible_equiv
 : Lemma ((base_heap.ghost_pts_to meta x v0 `base_heap.star` base_heap.ghost_pts_to meta x v1) ==
          (base_heap.ghost_pts_to meta x (op pcm v0 v1)))
 
+let heap_cell_evolves (h0 h1:option H.cell)
+: prop
+= match h0, h1 with
+  | None, None -> True
+  | None, Some (H.Ref meta _ _ _) -> reveal meta == false
+  | Some (H.Ref meta a p v), Some (H.Ref meta' a' p' v') ->
+    meta == meta' /\ (reveal meta ==> a==a' /\ p==p' /\ v==v')
+  | _, _ -> False
+
+let heaps_preserve_inames (m0 m1:base_heap.mem) =
+  ghost_ctr m0 <= ghost_ctr m1 /\
+  (forall (addr:nat).
+    heap_cell_evolves (select_ghost addr (core_of m0)) (select_ghost addr (core_of m1)))
+
+let preserves_inames 
+    (#a:Type u#a)
+    (#mg:bool)
+    (#pre:base_heap.slprop)
+    (#post:a -> GTot (base_heap.slprop))
+    (#ex:inames base_heap)
+    (action:_action_except (base_heap u#h) a mg ex pre post)
+= forall (m0:full_mem base_heap) frame. 
+    interpret (pre `base_heap.star` frame `base_heap.star` base_heap.mem_invariant ex m0) m0 /\
+    inames_ok ex m0
+    ==> ( 
+    let x, m1 = action frame m0 in
+    heaps_preserve_inames m0 m1
+    )
+
 val ghost_extend
     (meta:erased bool)
     (#ex:inames base_heap)
     (#a:Type u#a)
     (#pcm:pcm a)
     (x:erased a{pcm.refine x})
-: ghost_action_except base_heap (ghost_ref a pcm) ex    
-      base_heap.emp 
-      (fun r -> base_heap.ghost_pts_to meta r x)
+: act:ghost_action_except base_heap (ghost_ref a pcm) ex    
+        base_heap.emp 
+        (fun r -> base_heap.ghost_pts_to meta r x) {
+            reveal meta == false ==> preserves_inames act
+        }
 
 val ghost_extend_spec
       (#meta:bool)
@@ -84,9 +117,11 @@ val ghost_read
     (f:(v:a{compatible p x v}
         -> GTot (y:a{compatible p y v /\
                      FStar.PCM.frame_compatible p x v y})))
-: ghost_action_except base_heap (erased (v:a{compatible p x v /\ p.refine v})) ex
-    (base_heap.ghost_pts_to meta r x)
-    (fun v -> base_heap.ghost_pts_to meta r (f v))
+: act:ghost_action_except base_heap (erased (v:a{compatible p x v /\ p.refine v})) ex
+        (base_heap.ghost_pts_to meta r x)
+        (fun v -> base_heap.ghost_pts_to meta r (f v)) {
+            preserves_inames act
+        }
 
 val ghost_write
     (#ex:inames base_heap)
@@ -96,9 +131,11 @@ val ghost_write
     (r:ghost_ref a p)
     (x y:Ghost.erased a)
     (f:FStar.PCM.frame_preserving_upd p x y)
-: ghost_action_except base_heap unit ex
-    (base_heap.ghost_pts_to meta r x)
-    (fun _ -> base_heap.ghost_pts_to meta r y)
+: act:ghost_action_except base_heap unit ex
+        (base_heap.ghost_pts_to meta r x)
+        (fun _ -> base_heap.ghost_pts_to meta r y) {
+            reveal meta == false ==> preserves_inames act
+        }
 
 val ghost_share
     (#ex:inames base_heap)
@@ -108,9 +145,12 @@ val ghost_share
     (r:ghost_ref a pcm)
     (v0:FStar.Ghost.erased a)
     (v1:FStar.Ghost.erased a{composable pcm v0 v1})
-: ghost_action_except base_heap unit ex
+: act:ghost_action_except base_heap unit ex
     (base_heap.ghost_pts_to meta r (v0 `op pcm` v1))
-    (fun _ -> base_heap.ghost_pts_to meta r v0 `base_heap.star` base_heap.ghost_pts_to meta r v1)
+    (fun _ -> base_heap.ghost_pts_to meta r v0 `base_heap.star` base_heap.ghost_pts_to meta r v1) {
+        preserves_inames act
+    }
+
 
 val ghost_gather
     (#ex:inames base_heap)
@@ -120,19 +160,22 @@ val ghost_gather
     (r:ghost_ref a pcm)
     (v0:FStar.Ghost.erased a)
     (v1:FStar.Ghost.erased a)
-: ghost_action_except base_heap (squash (composable pcm v0 v1)) ex
+: act:ghost_action_except base_heap (squash (composable pcm v0 v1)) ex
     (base_heap.ghost_pts_to meta r v0 `base_heap.star` base_heap.ghost_pts_to meta r v1)
-    (fun _ -> base_heap.ghost_pts_to meta r (op pcm v0 v1))
-
+    (fun _ -> base_heap.ghost_pts_to meta r (op pcm v0 v1)) {
+        preserves_inames act
+    }
 
 val extend
     (#ex:inames base_heap)
     (#a:Type u#a)
     (#pcm:pcm a)
     (x:a{pcm.refine x})
-: action_except base_heap (ref a pcm) ex    
-      base_heap.emp 
-      (fun r -> base_heap.pts_to r x)
+: act:action_except base_heap (ref a pcm) ex    
+        base_heap.emp 
+        (fun r -> base_heap.pts_to r x) {
+            preserves_inames act
+        }
 
 val read
     (#ex:inames base_heap)
@@ -143,9 +186,11 @@ val read
     (f:(v:a{compatible p x v}
         -> GTot (y:a{compatible p y v /\
                      FStar.PCM.frame_compatible p x v y})))
-: action_except base_heap (v:a{compatible p x v /\ p.refine v}) ex
+: act:action_except base_heap (v:a{compatible p x v /\ p.refine v}) ex
     (base_heap.pts_to r x)
-    (fun v -> base_heap.pts_to r (f v))
+    (fun v -> base_heap.pts_to r (f v)) {
+        preserves_inames act
+    }
 
 val write
     (#ex:inames base_heap)
@@ -154,9 +199,11 @@ val write
     (r:ref a p)
     (x y:Ghost.erased a)
     (f:FStar.PCM.frame_preserving_upd p x y)
-: action_except base_heap unit ex
+: act:action_except base_heap unit ex
     (base_heap.pts_to r x)
-    (fun _ -> base_heap.pts_to r y)
+    (fun _ -> base_heap.pts_to r y) {
+        preserves_inames act
+    }
 
 val share
     (#ex:inames base_heap)
@@ -165,9 +212,11 @@ val share
     (r:ref a pcm)
     (v0:FStar.Ghost.erased a)
     (v1:FStar.Ghost.erased a{composable pcm v0 v1})
-: ghost_action_except base_heap unit ex
+: act:ghost_action_except base_heap unit ex
     (base_heap.pts_to r (v0 `op pcm` v1))
-    (fun _ -> base_heap.pts_to r v0 `base_heap.star` base_heap.pts_to r v1)
+    (fun _ -> base_heap.pts_to r v0 `base_heap.star` base_heap.pts_to r v1) {
+        preserves_inames act
+    }
 
 val gather
     (#ex:inames base_heap)
@@ -176,9 +225,11 @@ val gather
     (r:ref a pcm)
     (v0:FStar.Ghost.erased a)
     (v1:FStar.Ghost.erased a)
-: ghost_action_except base_heap (squash (composable pcm v0 v1)) ex
+: act:ghost_action_except base_heap (squash (composable pcm v0 v1)) ex
     (base_heap.pts_to r v0 `base_heap.star` base_heap.pts_to r v1)
-    (fun _ -> base_heap.pts_to r (op pcm v0 v1))
+    (fun _ -> base_heap.pts_to r (op pcm v0 v1)) {
+        preserves_inames act
+    }
 
 val pts_to_not_null_action 
       (#ex:inames base_heap)
@@ -186,9 +237,11 @@ val pts_to_not_null_action
       (#pcm:pcm a)
       (r:erased (ref a pcm))
       (v:Ghost.erased a)
-: ghost_action_except base_heap (squash (not (is_null r))) ex
+: act:ghost_action_except base_heap (squash (not (is_null r))) ex
     (base_heap.pts_to r v)
-    (fun _ -> base_heap.pts_to r v)
+    (fun _ -> base_heap.pts_to r v) {
+        preserves_inames act
+    }
 
 val exists_congruence 
         (#a:Type u#a)
